src/proof/algebra/reserved_keys.v
@@ -1,0 +1,58 @@
+From New.proof Require Import prelude.
+From New.proof Require Export pure_objects.
+From New.ghost Require Import auth_set.
+
+Section reserved_keys.
+Context `{!allG Σ}.
+
+Definition own_auth γ (reserved_keys : gset KKey.t) : iProp Σ :=
+  auth_set_auth γ reserved_keys.
+
+Definition own_frag γ (key : KKey.t) : iProp Σ :=
+  auth_set_frag γ key.
+
+Global Instance own_auth_timeless γ reserved_keys :
+  Timeless (own_auth γ reserved_keys).
+Proof. unfold own_auth. apply _. Qed.
+
+Global Instance own_frag_timeless γ key :
+  Timeless (own_frag γ key).
+Proof. unfold own_frag. apply _. Qed.
+
+Lemma init :
+  ⊢ |==> ∃ γ, own_auth γ (∅ : gset KKey.t).
+Proof.
+  unfold own_auth.
+  apply auth_set_init.
+Qed.
+
+Lemma frag_elem_of_auth {γ reserved_keys} key :
+  own_auth γ reserved_keys -∗
+  own_frag γ key -∗
+  ⌜ key ∈ reserved_keys ⌝.
+Proof.
+  unfold own_auth, own_frag.
+  apply auth_set_elem.
+Qed.
+
+Lemma reserve_key_vs {γ reserved_keys} key :
+  key ∉ reserved_keys →
+  own_auth γ reserved_keys ==∗
+    own_auth γ ({[key]} ∪ reserved_keys) ∗
+    own_frag γ key.
+Proof.
+  unfold own_auth, own_frag.
+  apply auth_set_alloc.
+Qed.
+
+Lemma consume_reserved_key_vs {γ reserved_keys} key :
+  own_auth γ reserved_keys -∗
+  own_frag γ key ==∗
+    own_auth γ (reserved_keys ∖ {[key]}).
+Proof.
+  unfold own_auth, own_frag.
+  iIntros "Hauth Hfrag".
+  iApply (auth_set_dealloc with "[$Hauth $Hfrag]").
+Qed.
+
+End reserved_keys.
