src/proof/kubernetes_model/update_status.v
@@ -374,10 +374,14 @@ Proof.
   { iNamed "H".
     iFrame "#". iFrame. iPureIntro. split_and!.
     all: try done.
-    eapply update_tombed_uid_update_eq_used_uid_sub; [done|done|].
-    unfold new_kobj, new_kmeta.
-    rewrite objectmeta_update_objectmeta.
-    eapply valid_simple_update_updated_set_resource_version_uid; done.
+    - eapply update_tombed_uid_update_eq_used_uid_sub; [done|done|].
+      unfold new_kobj, new_kmeta.
+      rewrite objectmeta_update_objectmeta.
+      eapply valid_simple_update_updated_set_resource_version_uid; done.
+    - rewrite dom_insert_L.
+      assert (key ∈ dom abs_state) as Hkey_in_abs.
+      { apply elem_of_dom. eexists. exact Hlookup_abs. }
+      Timeout 10 set_solver.
   }
   iExact "HΦ".
 Unshelve.
